Full proof

src/5.1.lean
@@ -47,31 +47,49 @@ bind item func :=
   | COption.none => COption.none
   | COption.some arg => func arg
 
---Proof that the default instance of Option satisfies the
---monad contract
-example (f : α → COption β) (o : α):
-bind (pure o) f = f o := by{
-  rw [pure, Applicative.toPure, Monad.toApplicative,
-   instMonadCOption]
-  simp
-  rw [bind, Monad.toBind]
-}
 
---Again but using a dedicated Prop so i can prove the
---2nd part of the problem
 def monadContract (m : Type → Type) (α β : Type) [Monad m] : Prop :=
-∀ (f : α → m β) (o : α), bind (pure o) f = f o 
+-- pure should be a left identity of bind
+(∀(f : α → m β) (v : α), bind (pure v) f = f v) ∧ 
+--pure should be a right identity of bind
+(∀(v : m α), bind v pure = v) ∧
+--bind should be associative
+(∀(v : m α) (f : α → m β) (g : β → m α), 
+  bind (bind v f) g = bind v (fun x => bind (f x) g))
 
-#check @monadContract
-
---COption satisfies the monad contract
-example {α β : Type}: monadContract COption α β
+--COption satisfies the monad contract, for real
+example {α β : Type}: monadContract COption α β 
 := by{
-  rw [monadContract, pure, Applicative.toPure,
-      Monad.toApplicative, instMonadCOption]
-  simp
-  rw [bind, Monad.toBind]
-  simp
+  rw [monadContract]
+  apply And.intro{
+    --left identity
+    intros f v;
+    rw [pure, Applicative.toPure, Monad.toApplicative,
+      instMonadCOption]
+    simp
+    rw [bind, Monad.toBind]
+  }
+  apply And.intro{
+    --right identity
+    intros v;
+    rw [bind, Monad.toBind, instMonadCOption]
+    simp;
+    cases v;{
+      trivial;
+    }{
+      trivial;
+    }
+  }{
+    --associative
+    intros v f g;
+    rw [bind, Monad.toBind, instMonadCOption];
+    simp;
+    cases v;{
+      trivial;
+    }{
+      trivial;
+    }
+  }
 }
 
 inductive BOption (α : Type) : Type
@@ -79,38 +97,12 @@ inductive BOption (α : Type) : Type
 | some : α -> BOption α
 
 instance : Monad BOption where
-pure arg := BOption.some arg
-bind _ _ := BOption.none
+  pure arg := BOption.some arg
+  bind _ _ := BOption.none
 
-#check Exists.intro
-
---Some random lemmas I was using for this
-
---This is such a jank proof of this lmao
-theorem L1 (α : Type) (p : α->Prop) :
-(¬∀(x : α),p x) <-> (∃(x : α),¬(p x))
-:= by{
-  rw [Not];
-  apply Iff.intro{
-    intro H;
-    apply Classical.byContradiction;
-    intro H2;
-    rw [Not] at H2;
-    apply H;
-    intro x;
-    apply Classical.byContradiction;
-    intro H3;
-    apply H2;
-    apply Exists.intro x;
-    exact H3;
-  }{
-    intros H1 H2;
-    apply Exists.elim H1;
-    intros x npx;
-    have H3 := H2 x;
-    trivial
-  }
-} 
+#check Option
+#check bind
+#check pure
 
 theorem L2: ∀(p : Prop), ¬¬p <-> p :=
 by{
@@ -132,25 +124,22 @@ by{
   }
 }  
 
---Proof BOption does not satisfy the monad contract. I'm 
---only able to prove this so far assuming β and α are nonempty types
-example {α β : Type} [iβ : Nonempty β] [iα : Nonempty α]:
-¬monadContract BOption α β
+--[iβ : Nonempty β] [iα : Nonempty α]
+example {α β : Type} [iα : Nonempty α]:
+¬monadContract BOption α β 
 := by{
-  rw [monadContract];
-  rewrite [L1];
-  have b := @Classical.choice β iβ;
-  let f1 := (fun (_ : α) => BOption.some b);
-  apply Exists.intro f1;
-  rewrite [L1];
-  have a := @Classical.choice α iα;
-  apply Exists.intro a;
-  rw [Not]
-  intro H;
-  rw [pure, Applicative.toPure,
-      Monad.toApplicative, instMonadBOption] at H;
-  simp at H;
+  unhygienic
+  apply Classical.byContradiction _;
+  intros H;
+  rw [L2] at H;
+  rw [monadContract] at H;
+  cases H;
+  cases right;
+  have H2 := left_1 (BOption.some (Classical.choice iα));
+  rw [bind, Monad.toBind, instMonadBOption] at H2;
+  simp at H2;
 }
+
 
 
 
@@ -188,3 +177,79 @@ example {α β : Type} [iβ : Nonempty β] [iα : Nonempty α]:
 --   }
 -- }
 
+--Proof that the default instance of Option satisfies the
+--monad contract (or at least part of it lmao)
+example (f : α → COption β) (o : α):
+bind (pure o) f = f o := by{
+  rw [pure, Applicative.toPure, Monad.toApplicative,
+   instMonadCOption]
+  simp
+  rw [bind, Monad.toBind]
+}
+
+--Again but using a dedicated Prop so i can prove the
+--2nd part of the problem
+def monadContractLeft (m : Type → Type) (α β : Type) [Monad m] : Prop :=
+∀ (f : α → m β) (o : α), bind (pure o) f = f o
+
+#check @monadContract
+
+--COption satisfies the monad contract
+example {α β : Type}: monadContractLeft COption α β
+:= by{
+  rw [monadContractLeft, pure, Applicative.toPure,
+      Monad.toApplicative, instMonadCOption]
+  simp
+  rw [bind, Monad.toBind]
+  simp
+}
+
+#check Exists.intro
+
+--Some random lemmas I was using for this
+
+--This is such a jank proof of this lmao
+theorem L1 (α : Type) (p : α->Prop) :
+(¬∀(x : α),p x) <-> (∃(x : α),¬(p x))
+:= by{
+  rw [Not];
+  apply Iff.intro{
+    intro H;
+    apply Classical.byContradiction;
+    intro H2;
+    rw [Not] at H2;
+    apply H;
+    intro x;
+    apply Classical.byContradiction;
+    intro H3;
+    apply H2;
+    apply Exists.intro x;
+    exact H3;
+  }{
+    intros H1 H2;
+    apply Exists.elim H1;
+    intros x npx;
+    have H3 := H2 x;
+    trivial
+  }
+} 
+
+--Proof BOption does not satisfy the monad contract. I'm 
+--only able to prove this so far assuming β and α are nonempty types
+example {α β : Type} [iβ : Nonempty β] [iα : Nonempty α]:
+¬monadContractLeft BOption α β
+:= by{
+  rw [monadContractLeft];
+  rewrite [L1];
+  have b := @Classical.choice β iβ;
+  let f1 := (fun (_ : α) => BOption.some b);
+  apply Exists.intro f1;
+  rewrite [L1];
+  have a := @Classical.choice α iα;
+  apply Exists.intro a;
+  rw [Not]
+  intro H;
+  rw [pure, Applicative.toPure,
+      Monad.toApplicative, instMonadBOption] at H;
+  simp at H;
+}
